converted alphabets to finite and added finiteness proof for PDA_To_CFG

TaskinBA/PDA_To_CFG.thy
@@ -6,6 +6,15 @@ datatype ('q, 's) pda_nt = Start_sym | Single_sym 'q 's 'q | List_sym 'q "'s lis
 
 context pda begin
 
+abbreviation all_pushes :: "'s list set" where 
+"all_pushes \<equiv> {\<alpha>| p \<alpha> q a z. (p, \<alpha>) \<in> trans_fun M q a z} \<union> {\<alpha>| p \<alpha> q z. (p, \<alpha>) \<in> eps_fun M q z}"
+
+abbreviation max_push :: nat where 
+"max_push \<equiv> Suc (Max (length ` all_pushes))"
+
+abbreviation is_allowed_nt :: "('q, 's) pda_nt set" where 
+"is_allowed_nt \<equiv> {List_sym p \<alpha> q| p \<alpha> q. length \<alpha> \<le> max_push} \<union> (\<Union>p Z q. {Single_sym p Z q}) \<union> {Start_sym}"
+
 abbreviation empty_rule :: "'q \<Rightarrow> (('q, 's) pda_nt, 'a) Prods" where
   "empty_rule q \<equiv> {(List_sym q [] q, [])}"
 
@@ -24,10 +33,80 @@ abbreviation start_rule :: "'q \<Rightarrow> (('q, 's) pda_nt, 'a) Prods" where
 
 abbreviation rule_set :: "(('q, 's) pda_nt, 'a) Prods" where
   "rule_set \<equiv> (\<Union>q. empty_rule q) \<union> (\<Union>q p a Z. trans_rule q p a Z) \<union> (\<Union>q p Z. eps_rule q p Z) \<union> 
-                 (\<Union>q nt. split_rule q nt) \<union> (\<Union>q. start_rule q)"
+                 \<Union> {split_rule q nt| q nt. nt \<in> is_allowed_nt} \<union> (\<Union>q. start_rule q)"
 
 definition G :: "(('q, 's) pda_nt,'a) Cfg" where
   "G \<equiv> Cfg rule_set Start_sym"
+
+lemma finite_is_allowed_nt: "finite (is_allowed_nt)"
+proof (intro finite_UnI)
+  show "finite {List_sym (p :: 'q) (\<alpha> :: 's list) q| p \<alpha> q. length \<alpha> \<le> max_push}"
+  proof -
+    let ?A = "\<Union>(\<Union>((\<lambda>s. (\<lambda>f. f ` UNIV) ` s) ` ((\<lambda>f. f ` {xs :: 's list. set xs \<subseteq> UNIV \<and> length xs \<le> max_push}) ` (List_sym ` (UNIV :: 'q set)))))"
+
+    have "{List_sym p \<alpha> q| p \<alpha> q. length \<alpha> \<le> max_push} = ?A"
+      by auto
+
+    moreover have "finite ?A" (is "finite (\<Union>?B)")
+    proof (rule finite_Union)
+      show "finite ?B" (is "finite (\<Union>?C)")
+      proof (rule finite_Union)
+        show "finite ?C" by simp
+      next
+        show "\<And>M. M \<in> ?C \<Longrightarrow> finite M" 
+          using finite_lists_length_le[of UNIV max_push] by force
+      qed
+    next
+      show "\<And>M. M \<in> ?B \<Longrightarrow> finite M" by fastforce
+    qed
+
+    ultimately show ?thesis by simp
+  qed
+next
+  show "finite (\<Union>(p :: 'q) (Z :: 's) q. {Single_sym p Z q})"
+    by (rule, simp)+
+qed simp
+
+lemma finite_split_rule: "finite (split_rule q nt)"
+  by (induction q nt rule: split_rule.induct) auto
+
+lemma "finite (Prods G)"
+proof -
+  have "finite (\<Union>q. empty_rule q)" by simp
+
+  moreover have "finite (\<Union>q p a Z. trans_rule q p a Z)"
+    by (simp add: finite_trans)
+
+  moreover have "finite (\<Union>q p Z. eps_rule q p Z)"
+    by (simp add: finite_eps)
+
+  moreover have "finite (\<Union> {split_rule q nt| q nt. nt \<in> is_allowed_nt})"
+  proof -
+    have "{split_rule q nt| q nt. nt \<in> is_allowed_nt} = \<Union> ((\<lambda>f. f ` is_allowed_nt) ` (split_rule ` UNIV))"
+      by fastforce
+
+    moreover have "finite (\<Union> (\<Union> ((\<lambda>f. f ` is_allowed_nt) ` (split_rule ` UNIV))))" (is "finite (\<Union>?A)")
+    proof (rule finite_Union)
+      show "finite ?A" (is "finite (\<Union>?B)")
+      proof (rule finite_Union)
+        show "finite ?B" by simp
+      next
+        show "\<And>M. M \<in> ?B \<Longrightarrow> finite M"
+          using finite_is_allowed_nt by blast
+      qed
+    next
+      show "\<And>M. M \<in> ?A \<Longrightarrow> finite M"
+        by (auto simp: finite_split_rule)
+    qed
+
+    ultimately show ?thesis by simp
+  qed
+
+  moreover have "finite (\<Union>q. start_rule q)" by simp
+
+  ultimately show ?thesis
+    by (simp add: G_def)
+qed
 
 lemma split_rule_simp:
   "(A, w) \<in> split_rule q nt \<longleftrightarrow> (\<exists>p\<^sub>0 Z \<alpha> p\<^sub>1. nt = (List_sym p\<^sub>0 (Z#\<alpha>) p\<^sub>1) \<and> 
@@ -38,9 +117,52 @@ lemma pda_to_cfg_derive_empty:
   "Prods G \<turnstile> [Nt (List_sym p\<^sub>1 [] p\<^sub>2)] \<Rightarrow> x \<longleftrightarrow> p\<^sub>2 = p\<^sub>1 \<and> x = []"
 unfolding G_def using derive_singleton[of rule_set] split_rule_simp by auto
 
+lemma finite_all_pushes: "finite all_pushes"
+proof -
+  let ?A = "(\<lambda>(p, \<alpha>). \<alpha>) ` (\<Union>q a Z. trans_fun M q a Z \<union> (\<Union>q Z. eps_fun M q Z))" 
+  have "all_pushes = ?A" by fast
+
+  moreover have "finite ?A" 
+    by (rule, simp add: finite_trans finite_eps)+
+
+  ultimately show ?thesis by simp
+qed
+
+lemma push_trans_leq_max:
+  "(p, \<alpha>) \<in> trans_fun M q a Z \<Longrightarrow> length \<alpha> \<le> max_push"
+proof -
+  have "(p, \<alpha>) \<in> trans_fun M q a Z \<Longrightarrow> length \<alpha> \<le> Max (length ` all_pushes)" 
+    apply (rule Max_ge) using finite_all_pushes by blast+
+  thus "(p, \<alpha>) \<in> trans_fun M q a Z \<Longrightarrow> length \<alpha> \<le> max_push" by simp
+qed
+
+lemma push_eps_leq_max:
+  "(p, \<alpha>) \<in> eps_fun M q Z \<Longrightarrow> length \<alpha> \<le> max_push"
+proof -
+  have "(p, \<alpha>) \<in> eps_fun M q Z \<Longrightarrow> length \<alpha> \<le> Max (length ` all_pushes)"
+    apply (rule Max_ge) using finite_all_pushes by blast+
+  thus "(p, \<alpha>) \<in> eps_fun M q Z \<Longrightarrow> length \<alpha> \<le> max_push" by simp
+qed
+
 lemma pda_to_cfg_derive_split:
-  "Prods G \<turnstile> [Nt (List_sym p\<^sub>1 (Z#\<alpha>) p\<^sub>2)] \<Rightarrow> w \<longleftrightarrow> (\<exists>q. w = [Nt (Single_sym p\<^sub>1 Z q), Nt (List_sym q \<alpha> p\<^sub>2)])"
-unfolding G_def using derive_singleton[of rule_set] split_rule_simp by auto
+ "Prods G \<turnstile> [Nt (List_sym p\<^sub>1 (Z#\<alpha>) p\<^sub>2)] \<Rightarrow> w \<longleftrightarrow> (\<exists>q. length (Z#\<alpha>) \<le> max_push \<and> w = [Nt (Single_sym p\<^sub>1 Z q), Nt (List_sym q \<alpha> p\<^sub>2)])"
+(is "?l \<longleftrightarrow> ?r")
+proof
+  assume ?l
+  hence "(List_sym p\<^sub>1 (Z # \<alpha>) p\<^sub>2, w) \<in> rule_set"
+    using derive_singleton[of "Prods G" "Nt (List_sym p\<^sub>1 (Z # \<alpha>) p\<^sub>2)" w] by (simp add: G_def)
+  thus ?r
+    by (auto simp: split_rule_simp)
+next
+  assume ?r
+  then obtain q where len_\<alpha>: "length (Z#\<alpha>) \<le> max_push" and w_def: "w = [Nt (Single_sym p\<^sub>1 Z q), Nt (List_sym q \<alpha> p\<^sub>2)]" by blast
+  from w_def have "(List_sym p\<^sub>1 (Z#\<alpha>) p\<^sub>2, w) \<in> split_rule q (List_sym p\<^sub>1 (Z # \<alpha>) p\<^sub>2)" by simp
+  with len_\<alpha> have "(List_sym p\<^sub>1 (Z#\<alpha>) p\<^sub>2, w) \<in> \<Union> {split_rule q nt| q nt. nt \<in> is_allowed_nt}"
+    by (subst Union_iff) fast
+  hence "(List_sym p\<^sub>1 (Z#\<alpha>) p\<^sub>2, w) \<in> rule_set" by simp
+  thus ?l
+    using derive_singleton[of "Prods G" "Nt (List_sym p\<^sub>1 (Z # \<alpha>) p\<^sub>2)" w] by (simp add: G_def)
+qed
 
 lemma pda_to_cfg_derive_single:
 "Prods G \<turnstile> [Nt (Single_sym q\<^sub>0 Z q\<^sub>1)] \<Rightarrow> w \<longleftrightarrow> 
@@ -54,7 +176,8 @@ unfolding G_def using derive_singleton[of rule_set] split_rule_simp by auto
 
 lemma pda_to_cfg_derives_if_stepn:
   assumes "stepn n (q, x, \<gamma>) (p, [], [])"
-  shows "Prods G \<turnstile> [Nt (List_sym q \<gamma> p)] \<Rightarrow>* map Tm x"
+      and "length \<gamma> \<le> max_push"
+    shows "Prods G \<turnstile> [Nt (List_sym q \<gamma> p)] \<Rightarrow>* map Tm x"
 using assms proof (induction n arbitrary: x p q \<gamma> rule: less_induct)
   case (less n)
   then show ?case proof (cases \<gamma>)
@@ -83,8 +206,10 @@ using assms proof (induction n arbitrary: x p q \<gamma> rule: less_induct)
         using split_stack[of n' q' x' \<beta> \<alpha> p] by blast
       from n_def m1_m2_n' have m1_less_n: "m\<^sub>1 < n" by simp
       from n_def m1_m2_n' have m2_less_n: "m\<^sub>2 < n" by simp
+      from eps have len_\<beta>: "length \<beta> \<le> max_push"
+        using push_eps_leq_max by blast
 
-      from Cons have "Prods G \<turnstile> [Nt (List_sym q \<gamma> p)] \<Rightarrow> [Nt (Single_sym q Z p'), Nt (List_sym p' \<alpha> p)]"
+      from Cons less(3) have "Prods G \<turnstile> [Nt (List_sym q \<gamma> p)] \<Rightarrow> [Nt (Single_sym q Z p'), Nt (List_sym p' \<alpha> p)]"
         using pda_to_cfg_derive_split by simp
 
       moreover from eps have "Prods G \<turnstile> [Nt (Single_sym q Z p'), Nt (List_sym p' \<alpha> p)] \<Rightarrow> 
@@ -93,9 +218,9 @@ using assms proof (induction n arbitrary: x p q \<gamma> rule: less_induct)
                                                             "[Nt (List_sym p' \<alpha> p)]"] by simp
       
       moreover have "Prods G \<turnstile> [Nt (List_sym q' \<beta> p'), Nt (List_sym p' \<alpha> p)] \<Rightarrow>* map Tm y @ [Nt (List_sym p' \<alpha> p)]"
-        using derives_append[OF less(1)[OF m1_less_n stepm1]] by simp
+        using derives_append[OF less(1)[OF m1_less_n stepm1 len_\<beta>]] by simp
 
-      moreover from x_def x'_def have "Prods G \<turnstile> map Tm y @ [Nt (List_sym p' \<alpha> p)] \<Rightarrow>* map Tm x"
+      moreover from x_def x'_def Cons less(3) have "Prods G \<turnstile> map Tm y @ [Nt (List_sym p' \<alpha> p)] \<Rightarrow>* map Tm x"
         using derives_prepend[OF less(1)[OF m2_less_n stepm2]] by auto
 
       ultimately show ?thesis by simp
@@ -107,8 +232,10 @@ using assms proof (induction n arbitrary: x p q \<gamma> rule: less_induct)
         using split_stack[of n' q' x' \<beta> \<alpha> p] by blast
       from n_def m1_m2_n' have m1_less_n: "m\<^sub>1 < n" by simp
       from n_def m1_m2_n' have m2_less_n: "m\<^sub>2 < n" by simp
+      from trans have len_\<beta>: "length \<beta> \<le> max_push"
+        using push_trans_leq_max by blast
 
-      from Cons have "Prods G \<turnstile> [Nt (List_sym q \<gamma> p)] \<Rightarrow> [Nt (Single_sym q Z p'), Nt (List_sym p' \<alpha> p)]"
+      from Cons less(3) have "Prods G \<turnstile> [Nt (List_sym q \<gamma> p)] \<Rightarrow> [Nt (Single_sym q Z p'), Nt (List_sym p' \<alpha> p)]"
         using pda_to_cfg_derive_split by simp
 
       moreover from trans have "Prods G \<turnstile> [Nt (Single_sym q Z p'), Nt (List_sym p' \<alpha> p)] \<Rightarrow>
@@ -118,9 +245,9 @@ using assms proof (induction n arbitrary: x p q \<gamma> rule: less_induct)
 
       moreover have "Prods G \<turnstile> [Tm a, Nt (List_sym q' \<beta> p'), Nt (List_sym p' \<alpha> p)] \<Rightarrow>*
                                       Tm a # map Tm y @ [Nt (List_sym p' \<alpha> p)]"
-        using derives_append[OF less(1)[OF m1_less_n stepm1]] by (simp add: derives_Tm_Cons)
+        using derives_append[OF less(1)[OF m1_less_n stepm1 len_\<beta>]] by (simp add: derives_Tm_Cons)
 
-      moreover from x'_def x_def have "Prods G \<turnstile> Tm a # map Tm y @ [Nt (List_sym p' \<alpha> p)] \<Rightarrow>* map Tm x"
+      moreover from x'_def x_def Cons less(3) have "Prods G \<turnstile> Tm a # map Tm y @ [Nt (List_sym p' \<alpha> p)] \<Rightarrow>* map Tm x"
         using derives_prepend[OF less(1)[OF m2_less_n stepm2], of "Tm a # map Tm y"] by simp
 
       ultimately show ?thesis by simp
